AlgoleanTests.lean
@@ -5,6 +5,8 @@ public import AlgoleanTests.FreeMonadWP
 public import AlgoleanTests.KMPExamples
 public import AlgoleanTests.ModelM
 public import AlgoleanTests.ModelMWP
+public import AlgoleanTests.ModelStateM
+public import AlgoleanTests.ModelStateMWP
 public import AlgoleanTests.NaivePatternSearchExamples
 public import AlgoleanTests.ProgExamples
 public import AlgoleanTests.QueryExamples
